Better stack bounds for Equal

compiler/backend/semantics/dataSemScript.sml
@@ -38,7 +38,7 @@ val _ = Datatype `
        stack_limit  : num;    (* max stack size *)
        arch_64_bit  : bool;   (* the arch is either 64-bit or 32-bit *)
        has_fp_ops   : bool;   (* the arch supports float ops *)
-       has_fp_tops  : bool    (* the arch supports float ops *)                        
+       has_fp_tops  : bool    (* the arch supports float ops *)
        |> `
 
 val _ = Datatype `
@@ -241,12 +241,12 @@ val vb_size_def = tDefine"vb_size"`
  ntac 2 gen_tac \\ Induct \\ rw[fetch "-" "v_size_def"] \\ rw[]
  \\ res_tac \\ rw[]);
 
-val vc_size_def = tDefine"vc_size"`
-  (vc_size (Block ts t ls) = 1 + SUM (MAP vc_size ls) + LENGTH ls) ∧
-  (vc_size _ = 1n)`
-(WF_REL_TAC`measure v_size` \\
- ntac 2 gen_tac \\ Induct \\ rw[fetch "-" "v_size_def"] \\ rw[]
- \\ res_tac \\ rw[]);
+val vs_depth_def = tDefine"vs_depth"`
+  (vs_depth (Block ts t ls) = vs_depth_list ls) ∧
+  (vs_depth _ = 0) ∧
+  (vs_depth_list [] = 0) ∧
+  (vs_depth_list (x::xs) = MAX (1 + vs_depth x) (vs_depth_list xs))`
+(WF_REL_TAC`measure (λx. sum_CASE x v_size v1_size)`);
 
 Definition eq_code_stack_max_def:
   eq_code_stack_max n tsz =
@@ -311,7 +311,7 @@ val stack_consumed_def = Define `
       small_enough_int (n1 * n2) then
      SOME 0 else NONE) /\
   (stack_consumed sfs lims (Equal) vs =
-   (eq_code_stack_max (vc_size (HD vs) + 1) sfs)) /\
+   (eq_code_stack_max (vs_depth (HD vs) + 1) sfs)) /\
   (stack_consumed sfs lims (Sub) [Number n1; Number n2] =
    if small_enough_int n1 /\
       small_enough_int n2 /\
