compiler/backend/proofs/data_to_word_memoryProofScript.sml
@@ -8407,104 +8407,6 @@ Proof
     \\ fs[] \\ rveq \\ fs[] \\ rfs [] )
 QED
 
-Theorem memory_rel_pointer_eq_vc_size:
-   ∀v1 v2 w.
-   good_dimindex (:'a) ∧
-   memory_rel c be ts refs sp st m dm ((v1,(w:'a word_loc))::(v2,w)::vars) ==>
-     vc_size v1 = vc_size v2
-Proof
-  ho_match_mp_tac v_ind \\ rw[] \\ Cases_on`v2` \\ fs[vc_size_def]
-  \\ qhdtm_x_assum`memory_rel`mp_tac
-  \\ qid_spec_tac`n` \\ qid_spec_tac`n0` \\ qid_spec_tac`n'`
-  THEN_LT USE_SG_THEN (fn th => metis_tac[memory_rel_swap,th]) 1 3
-  THEN_LT USE_SG_THEN (fn th => metis_tac[memory_rel_swap,th]) 2 3
-  THEN_LT USE_SG_THEN (fn th => metis_tac[memory_rel_swap,th]) 6 4
-  THEN_LT USE_SG_THEN (fn th => metis_tac[memory_rel_swap,th]) 6 4
-  \\ rw[]
-  >- (
-    Cases_on`small_int (:'a) i`
-    >- (
-      rpt_drule memory_rel_Number_IMP
-      \\ rpt_drule memory_rel_tail \\ strip_tac
-      \\ rpt_drule memory_rel_Block_IMP \\ strip_tac
-      \\ strip_tac \\ rveq \\ fs[] \\ rveq
-      \\ fs[Smallnum_0]
-      \\ `Smallnum i ' 1`
-      by (
-        `1 < dimindex (:'a)` by fs[good_dimindex_def]
-        \\ simp[Once WORD_ADD_BIT]
-        \\ simp[word_index,word_mul_n2w]
-        \\ `¬BIT 1 (n * 2 ** 4)`
-        by ( match_mp_tac bitTheory.BIT_SHIFT_THM3 \\ simp[] )
-        \\ fs[]
-        \\ simp[word_bits_n2w,word_index]
-        \\ match_mp_tac bitTheory.BIT_OF_BITS_THM2
-        \\ simp[] )
-      \\ rfs[Smallnum_1] )
-    \\ rpt_drule memory_rel_Number_bignum_IMP
-    \\ rpt_drule memory_rel_tail \\ strip_tac
-    \\ rpt_drule memory_rel_Block_IMP \\ strip_tac
-    \\ strip_tac \\ rveq \\ fs[] \\ rveq \\ fs[]
-    \\ qmatch_assum_rename_tac`(1w && w1) <> 0w`
-    \\ `word_bit 0 w1` by simp[word_bit_test]
-    \\ pop_assum mp_tac \\ rw[word_bit_thm] \\ fs[]
-    \\ rfs[word_bit_test] )
-  >- (
-    rpt_drule memory_rel_Word64_IMP
-    \\ rpt_drule memory_rel_tail \\ strip_tac
-    \\ rpt_drule memory_rel_Block_IMP \\ strip_tac
-    \\ strip_tac
-    \\ rveq \\ fs[] \\ rveq \\ fs[] \\ rveq \\ fs[]
-    \\ fs[get_addr_0] )
-  >- (
-    rpt_drule memory_rel_Block_IMP \\ strip_tac
-    \\ imp_res_tac memory_rel_tail
-    \\ rpt_drule memory_rel_Block_IMP \\ strip_tac
-    \\ clean_tac
-    \\ qmatch_asmsub_rename_tac`Word w`
-    \\ reverse(Cases_on`w ' 0` \\ fs[])
-    \\ fs[] \\ rveq \\ fs[] \\ rveq \\ fs[]
-    \\ imp_res_tac encode_header_tag_mask \\ fs[]
-    \\ fs[encode_header_def]
-    \\ fs[X_LT_DIV,LEFT_ADD_DISTRIB] \\ rfs[] \\ rveq
-    \\ `LENGTH l < dimword(:'a) ∧ LENGTH l' < dimword(:'a)`
-    by (
-      metis_tac[dimword_def,bitTheory.EXP_SUB_LESS_EQ,LESS_LESS_EQ_TRANS] )
-    \\ fs[]
-    \\ AP_TERM_TAC
-    \\ simp[LIST_EQ_REWRITE,EL_MAP]
-    \\ fs[] \\ qx_gen_tac`i` \\ strip_tac
-    \\ clean_tac
-    \\ qhdtm_x_assum`memory_rel`kall_tac
-    \\ rpt_drule memory_rel_Block_MEM \\ rw[]
-    \\ qmatch_assum_abbrev_tac`memory_rel _ _ _ _ _ _ _ _ (e1::b1::b2::vars)`
-    \\ `memory_rel c be ts refs sp st m dm (b2::e1::vars)`
-    by (
-      qhdtm_x_assum`memory_rel`mp_tac
-      \\ match_mp_tac memory_rel_rearrange
-      \\ rw[] \\ rw[] )
-    \\ unabbrev_all_tac
-    \\ `i < LENGTH l'` by simp[]
-    \\ rpt_drule memory_rel_Block_MEM \\ strip_tac
-    \\ rpt_drule memory_rel_swap \\ strip_tac
-    \\ rpt_drule memory_rel_tail \\ strip_tac
-    \\ fs[EVERY_MEM,MEM_EL,PULL_EXISTS,LIST_REL_EL_EQN]
-    \\ first_x_assum(match_mp_tac o MP_CANON) \\ simp[]
-    \\ rpt_drule memory_rel_swap \\ strip_tac
-    \\ asm_exists_tac \\ rw[] )
-  >- (
-    fs[memory_rel_def,word_ml_inv_def,abs_ml_inv_def,bc_stack_ref_inv_def]
-    \\ fs[v_inv_def] \\ rveq
-    \\ fs[word_addr_def]
-    \\ every_case_tac \\ fs[] \\ rveq \\ fs[word_addr_def])
-  >- (
-    rpt_drule memory_rel_RefPtr_IMP
-    \\ rpt_drule memory_rel_tail \\ strip_tac
-    \\ rpt_drule memory_rel_Block_IMP \\ strip_tac
-    \\ strip_tac
-    \\ fs[] \\ rveq \\ fs[] \\ rfs [] )
-QED
-
 val do_eq_list_F_IMP_MEM = prove(
   ``!l l'.
       do_eq_list refs l l' = Eq_val F /\ LENGTH l' = LENGTH l ==>
@@ -8971,6 +8873,12 @@ val word_is_clos_def = Define `
     (h && (tag_mask c || 2w)) = n2w (16 * closure_tag + 2) \/
     (h && (tag_mask c || 2w)) = n2w (16 * partial_app_tag + 2)`;
 
+(* l  corresponds to the functional big-step semantics clock.
+      Used to show that equality comparisons respect the
+      MustTerminate limit.
+   ck is an upper bound on the number of stack frames
+      allocated by an equality comparison.
+  *)
 val word_eq_def = tDefine "word_eq" `
   (word_eq c st dm m l ck w1 (w2:'a word) =
      if w1 = w2 then SOME (1w:'a word,l,ck) else
@@ -8980,8 +8888,8 @@ val word_eq_def = tDefine "word_eq" `
            if (h1 && 0b1100w) = 0w (* is Block *) then
              if word_is_clos c h1 (* isClos *) then SOME (1w,l,ck) else
              if ~(h1 = h2) then SOME (0w,l,ck) else
-             if l = 0 \/ ck = 0 then NONE else
-               word_eq_list c st dm m (l-1) (ck-1) (decode_length c h1)
+             if l = 0(* \/ ck = 0 *)then NONE else
+               word_eq_list c st dm m (l-1) ck (decode_length c h1)
                  (a1+bytes_in_word) (a2+bytes_in_word) else
            if ~(h1 = h2) then SOME (0w,l,ck) else
            if ~(word_bit 2 h1) (* is array *) then SOME (0w,l,ck) else
@@ -9004,14 +8912,14 @@ val word_eq_def = tDefine "word_eq" `
        | (Word w1, Word w2) =>
         (case fix_clock (ck-1) (l-1) (word_eq c st dm m (l-1) (ck-1) w1 w2) of
          | NONE => NONE
-         | SOME (x,l,ck) => if x <> 1w then SOME (x,l,ck) else
+         | SOME (x,l,ck') => if x <> 1w then SOME (x,l,ck) else
                             if l = 0 then NONE else
                               word_eq_list c st dm m (l-1) ck (w-1w)
                                 (a1 + bytes_in_word) (a2 + bytes_in_word))
        | _ => NONE)`
  (WF_REL_TAC `measure(\x. case x of
-                          | INL (c,st,dm,m,l1,ck1,w1,w2) => ck1
-                          | INR (c,st,dm,m,l1,ck1,w,a1,a2) => ck1)` >>
+                          | INL (c,st,dm,m,l1,ck1,w1,w2) => l1
+                          | INR (c,st,dm,m,l1,ck1,w,a1,a2) => l1)` >>
   rw[] >> imp_res_tac fix_clock_IMP >> rw[])
 
 val word_eq_ind = theorem "word_eq_ind";
@@ -9329,7 +9237,7 @@ Theorem word_eq_thm0:
        memory_rel c be ts refs sp st m dm
           ((v1,Word w1)::(v2,Word w2:'a word_loc)::vars) /\
        do_eq refs v1 v2 = Eq_val b /\
-       ck = vc_size v1 /\
+       ck = vs_depth v1 /\
        vb_size v1 * dimword (:'a) < l /\
        good_dimindex (:'a) ==>
        ?res l1 ck1. word_eq c st dm m l ck w1 w2 = SOME (res,l1,ck1) /\
@@ -9341,7 +9249,7 @@ Theorem word_eq_thm0:
        LENGTH v2 = LENGTH v1 /\ LENGTH v1 < dimword (:'a) /\
        eq_assum w1 m dm v1 /\ eq_assum w2 m dm v2 /\
        do_eq_list refs v1 v2 = Eq_val b /\
-       ck = (LENGTH v1 + SUM (MAP vc_size v1)) /\
+       ck = vs_depth_list v1 /\
        (LENGTH v1 + SUM (MAP vb_size v1)) * dimword (:'a) < l /\
        good_dimindex (:'a) ==>
        ?res l1 ck1. word_eq_list c st dm m l ck (n2w (LENGTH v1)) w1 w2 = SOME (res,l1,ck1) /\
@@ -9351,7 +9259,7 @@ Proof
   ho_match_mp_tac do_eq_ind \\ rpt conj_tac
   \\ once_rewrite_tac [do_eq_def] \\ simp []
   THEN1 (* do_eq Numbers *)
-   (rw [] \\ fs [vb_size_def,vc_size_def]
+   (rw [] \\ fs [vb_size_def,vs_depth_def]
     \\ once_rewrite_tac [word_eq_def]
     \\ IF_CASES_TAC
     THEN1 (rveq
@@ -9388,7 +9296,7 @@ Proof
     \\ rw [] \\ fs [word_cmp_res_def] \\ rw []
     \\ fs [good_dimindex_def] \\ rw [dimword_def])
   THEN1 (* do_eq Word64 *)
-   (rw [] \\ fs [vb_size_def,vc_size_def]
+   (rw [] \\ fs [vb_size_def,vs_depth_def]
     \\ once_rewrite_tac [word_eq_def]
     \\ IF_CASES_TAC
     THEN1 (rveq
@@ -9453,7 +9361,7 @@ Proof
       \\ simp[] \\ strip_tac \\ fs[]
       \\ clean_tac \\ strip_tac \\  fs[] )
     \\ clean_tac \\ fs[]
-    \\ fs[vb_size_def,vc_size_def]
+    \\ fs[vb_size_def,vs_depth_def]
     \\ imp_res_tac memory_rel_RefPtr_IMP_lemma \\ fs[]
     \\ `∃bs1 bs2.
           lookup n1 refs = SOME (ByteArray T bs1) ∧
@@ -9578,7 +9486,7 @@ Proof
     \\ first_x_assum drule \\ fs []
     \\ disch_then (qspec_then `l-1` mp_tac)
     \\ impl_tac THEN1
-     (fs [LEFT_ADD_DISTRIB,vb_size_def,vc_size_def]
+     (fs [LEFT_ADD_DISTRIB,vb_size_def,vs_depth_def]
       \\ qpat_x_assum `_ < l` mp_tac
       \\ CONV_TAC (DEPTH_CONV ETA_CONV)
       \\ Cases_on `l` \\ fs []
@@ -9586,9 +9494,8 @@ Proof
       \\ fs [encode_header_def]
       \\ fs [good_dimindex_def,dimword_def] \\ rfs [])
     \\ strip_tac \\ fs []
-    \\ drule_then(qspec_then `t1` assume_tac) (CONJUNCT2 word_eq_add_clock)
-    \\ fs[ETA_THM]
-    \\ fs [LEFT_ADD_DISTRIB,vb_size_def,vc_size_def]
+    \\ rw[vs_depth_def]
+    \\ fs [LEFT_ADD_DISTRIB,vb_size_def,vs_depth_def]
     \\ CONV_TAC (DEPTH_CONV ETA_CONV)
     \\ fs [good_dimindex_def,dimword_def] \\ rfs []
    )
@@ -9617,24 +9524,48 @@ Proof
   \\ disch_then (qspec_then `l-1` mp_tac)
   \\ impl_tac THEN1 fs [LEFT_ADD_DISTRIB]
   \\ strip_tac \\ fs []
-  \\ drule_then(qspec_then `LENGTH v1' + SUM (MAP vc_size v1')` assume_tac) (CONJUNCT1 word_eq_add_clock)
-  \\ fs[]
-  \\ IF_CASES_TAC \\ fs []
-  THEN1 (fs [LEFT_ADD_DISTRIB])
-  \\ fs [GSYM word_add_n2w]
-  \\ qpat_x_assum `memory_rel c be ts refs sp st m dm _` kall_tac
-  \\ `memory_rel c be ts refs sp st m dm
-           (eq_explode (w1 + bytes_in_word) m dm v1' ++
-            eq_explode (w2 + bytes_in_word) m dm v2' ++ vars)` by
-   (first_x_assum (fn th => mp_tac th THEN match_mp_tac memory_rel_rearrange)
-    \\ fs [] \\ rw [] \\ fs [] \\ NO_TAC)
-  \\ first_x_assum drule \\ fs []
-  \\ disch_then (qspec_then `l1-1` mp_tac)
-  \\ impl_tac THEN1 fs [LEFT_ADD_DISTRIB]
-  \\ strip_tac
-  \\ drule_then(qspec_then `ck1` assume_tac) (CONJUNCT2 word_eq_add_clock)
-  \\ fs[ETA_THM]
-  \\ fs[LEFT_ADD_DISTRIB]
+  (*\\ drule_then(qspec_then `LENGTH v1' + SUM (MAP v_depth v1')` assume_tac) (CONJUNCT1 word_eq_add_clock)*)
+  \\ simp[vs_depth_def]
+  \\ reverse(rw[MAX_DEF])
+  >- (fs[]
+      \\ IF_CASES_TAC \\ fs []
+      THEN1 (fs [LEFT_ADD_DISTRIB])
+      \\ fs [GSYM word_add_n2w]
+      \\ qpat_x_assum `memory_rel c be ts refs sp st m dm _` kall_tac
+      \\ `memory_rel c be ts refs sp st m dm
+               (eq_explode (w1 + bytes_in_word) m dm v1' ++
+                eq_explode (w2 + bytes_in_word) m dm v2' ++ vars)` by
+       (first_x_assum (fn th => mp_tac th THEN match_mp_tac memory_rel_rearrange)
+        \\ fs [] \\ rw [] \\ fs [] \\ NO_TAC)
+      \\ first_x_assum drule \\ fs []
+      \\ disch_then (qspec_then `l1-1` mp_tac)
+      \\ impl_tac THEN1 fs [LEFT_ADD_DISTRIB]
+      \\ strip_tac
+      \\ drule_then(qspec_then `(vs_depth v1 + 1) - vs_depth_list v1'` mp_tac) (CONJUNCT2 word_eq_add_clock)
+      \\ fs[NOT_LESS] \\ strip_tac
+      \\ fs[ETA_THM]
+      \\ fs[LEFT_ADD_DISTRIB])
+  >- (drule_then(qspec_then `vs_depth_list v1' - (vs_depth v1 + 1)` mp_tac) (CONJUNCT1 word_eq_add_clock) >>
+      fs[] >> strip_tac >>
+      dxrule_then(qspec_then `1` mp_tac) (CONJUNCT1 word_eq_add_clock) >>
+      simp[] >> strip_tac >>
+      fs[]
+      \\ IF_CASES_TAC \\ fs []
+      THEN1 (fs [LEFT_ADD_DISTRIB])
+      \\ fs [GSYM word_add_n2w]
+      \\ qpat_x_assum `memory_rel c be ts refs sp st m dm _` kall_tac
+      \\ `memory_rel c be ts refs sp st m dm
+               (eq_explode (w1 + bytes_in_word) m dm v1' ++
+                eq_explode (w2 + bytes_in_word) m dm v2' ++ vars)` by
+       (first_x_assum (fn th => mp_tac th THEN match_mp_tac memory_rel_rearrange)
+        \\ fs [] \\ rw [] \\ fs [] \\ NO_TAC)
+      \\ first_x_assum drule \\ fs []
+      \\ disch_then (qspec_then `l1-1` mp_tac)
+      \\ impl_tac THEN1 fs [LEFT_ADD_DISTRIB]
+      \\ strip_tac
+      \\ fs[ETA_THM]
+      \\ fs[LEFT_ADD_DISTRIB]
+     )
 QED
 
 Theorem word_eq_thm:
@@ -9642,7 +9573,7 @@ Theorem word_eq_thm:
       ((v1,Word w1)::(v2,Word w2:'a word_loc)::vars) /\
     do_eq refs v1 v2 = Eq_val b /\ good_dimindex (:'a) ==>
     ?res l1 ck1.
-       word_eq c st dm m (MustTerminate_limit (:'a) - 1) (vc_size v1) w1 w2 = SOME (res,l1,ck1) /\
+       word_eq c st dm m (MustTerminate_limit (:'a) - 1) (vs_depth v1) w1 w2 = SOME (res,l1,ck1) /\
        (b <=> (res = 1w))
 Proof
   rw [] \\ imp_res_tac memory_rel_limit
